test.v
@@ -1,0 +1,10 @@
+Require Import String Program.
+Require Import term.
+Open Scope string_scope.
+
+
+Goal True.
+  set True.
+  constr P.
+  constr universe.
+Abort.
